compcertxo/Lifting.v
@@ -39,7 +39,6 @@ Section Lifting.
     |}%rel.
 End Lifting.
 
-
 Delimit Scope li_scope with li.
 Bind Scope li_scope with language_interface.
 Delimit Scope lts_scope with lts.
@@ -67,33 +66,37 @@ Definition no_perm_on (m: mem) (vars: block -> Z -> Prop): Prop :=
 
 Record krel {K1 K2: Type}: Type :=
   mk_krel {
-      Rk: K1 -> K2 -> Prop;
-      Rm: K1 -> mem -> Prop;
-      G: block -> Z -> Prop;
+      Rk: K1 -> K2 * mem -> Prop;    (* a simulation relation *)
+      G: block -> Z -> Prop;         (* private variables *)
 
+      Rkm '(k1, m1) '(k2, m2) :=
+        Rk k1 (k2, m2) /\ no_perm_on m1 G /\ Mem.extends m1 m2;
       G_unchanged:
-        forall k m1 m2,
-          Rm k m1 -> Mem.unchanged_on G m1 m2 -> Rm k m2;
+        forall k1 k2 m m',
+          Rk k1 (k2, m)  -> Mem.unchanged_on G m m' -> Rk k1 (k2, m');
     }.
 Arguments krel: clear implicits.
+
+Program Definition krel_comp {K1 K2 K3} (R1: krel K1 K2) (R2: krel K2 K3) :=
+  {|
+  Rk k1 '(k3, m3) := exists '(k2, m2), Rk R1 k1 (k2, m2) /\ Rk R2 k2 (k3, m3);
+  G b ofs := G R1 b ofs /\ G R2 b ofs;
+  |}.
+Next Obligation.
+Admitted.
 
 Section SIM_REL.
   Context {K1 K2} (R: krel K1 K2).
 
   Inductive kcc_ext_query: query (li_c @ K1) -> query (li_c @ K2) -> Prop :=
   | kcc_query_intro vf sg vargs1 vargs2 m1 m2 k1 k2:
-      Val.lessdef_list vargs1 vargs2 ->
-      Mem.extends m1 m2 ->
-      vf <> Vundef -> Rk R k1 k2 -> Rm R k1 m2 ->
-      no_perm_on m1 (G R) ->
+      Val.lessdef_list vargs1 vargs2 -> vf <> Vundef ->
+      Rkm R (k1, m1) (k2, m2) ->
       kcc_ext_query (cq vf sg vargs1 m1, k1) (cq vf sg vargs2 m2, k2).
 
   Inductive kcc_ext_reply: reply (li_c @ K1) -> reply (li_c @ K2) -> Prop :=
   | kcc_ext_reply_intro vres1 vres2 m1 m2 k1 k2:
-      Val.lessdef vres1 vres2 ->
-      Mem.extends m1 m2 ->
-      Rk R k1 k2 -> Rm R k1 m2 ->
-      no_perm_on m1 (G R) ->
+      Val.lessdef vres1 vres2 -> Rkm R (k1, m1) (k2, m2) ->
       kcc_ext_reply (cr vres1 m1, k1) (cr vres2 m2, k2).
 
   Program Definition kcc_ext :=
@@ -106,67 +109,113 @@ Section SIM_REL.
 
 End SIM_REL.
 
-Module Ksim.
-  Record ksim {K1 K2: Type} :=
-    mk_ksim {
-        L1: Smallstep.semantics li_null (li_c @ K1);
-        L2: Smallstep.semantics li_null (li_c @ K2);
-        R: krel K1 K2;
-
-        layer_sim: forward_simulation 1 (kcc_ext R) L1 L2;
-      }.
-  Arguments ksim: clear implicits.
-End Ksim.
-
-Definition lts_closed {liA liB} (L: semantics liA liB) :=
-  forall se s q, ~ (at_external (L se)) s q.
-
-Lemma li_null_closed {li} (L: semantics li_null li): lts_closed L.
-Proof.
-  unfold lts_closed.
-  intros. inversion q.
-Qed.
-
-Section LTS_CLOSED.
-
-  Context {liA liB} (L: semantics liA liB).
-  Context (HL: lts_closed L).
-
-  Variable liX: language_interface.
-  Definition lts' se: lts liX liB (state L) :=
-    {|
-    genvtype := genvtype (L se);
-    step ge := step (L se) ge;
-    valid_query := valid_query (L se);
-    initial_state := initial_state (L se);
-    at_external := fun s q => False;
-    after_external := fun q s r => False;
-    final_state := final_state (L se);
-    globalenv := globalenv (L se)
-    |}.
-  Definition closed_sem_conv :=
-    {|
-    skel := skel L;
-    activate se := lts' se;
-    |}.
-
-  (* TODO: proved equivalence *)
-End LTS_CLOSED.
-
 Require Import Clight.
+
+Inductive state_match {K1 K2} (R: krel K1 K2): rel (state * K1) (state * K2) :=
+| State_match f s k e te m1 m2 k1 k2:
+    Rkm R (k1, m1) (k2, m2) ->
+    state_match R (State f s k e te m1, k1) (State f s k e te m2, k2)
+| Callstate_match v vs k m1 m2 k1 k2:
+    (* less_def on arguments? *)
+    Rkm R (k1, m1) (k2, m2) ->
+    state_match R (Callstate v vs k m1, k1) (Callstate v vs k m2, k2)
+| Returnstate_match v k m1 m2 k1 k2:
+    Rkm R (k1, m1) (k2, m2) ->
+    state_match R (Returnstate v k m1, k1) (Returnstate v k m2, k2).
+
+Lemma clight_lifted {K1 K2} p R:
+  forward_simulation (kcc_ext R) (kcc_ext R)
+                     ((semantics1 p) @ K1) ((semantics1 p) @ K2).
+Proof.
+  constructor. econstructor; eauto. instantiate (1  := fun _ _ _ => _). cbn beta.
+  intros se ? [ ] [ ] Hsk.
+  apply forward_simulation_step with (match_states := state_match R).
+  - intros. simpl. admit.
+  -
+
+Admitted.
+
+Notation " 'layer' K " := (Smallstep.semantics li_null (li_c @ K)) (at level 1).
+
+Definition layer_sim {K1 K2: Type} (L1: layer K1) (L2: layer K2)
+           (R: krel K1 K2) := forward_simulation 1 (kcc_ext R) L1 L2.
+
+(* Section Layer_Lifting. *)
+(*   Variable K: Type. *)
+(*   Context {li state} (L: lts li_null li state). *)
+
+(*   Definition lifted_lts_layer: lts li_null (li @ K) (state * K) := *)
+(*     {| *)
+(*     genvtype := genvtype L; *)
+(*     step ge := step' K L ge; *)
+(*     valid_query := fun (q: query (li @ K)) => valid_query L (fst q); *)
+(*     initial_state := (initial_state L) * eq; *)
+(*     at_external '(s, _) := at_external L s; *)
+(*     after_external '(s, _) r '(s', _) := after_external L s r s'; *)
+(*     final_state := (final_state L) * eq; *)
+(*     globalenv := globalenv L *)
+(*     |}%rel. *)
+(* End Layer_Lifting. *)
+
+(* Definition lifted_semantics_layer {li} (K: Type) (L: semantics li_null li) := *)
+(*   {| *)
+(*   skel := skel L; *)
+(*   activate se := lifted_lts_layer K (L se); *)
+(*   |}. *)
+
+(* Notation "L @ K" := (lifted_semantics_layer K L): sem_scope. *)
+
+
+
+(* TODO: move this to somewhere else *)
+(* Definition lts_closed {liA liB} (L: Smallstep.semantics liA liB) := *)
+(*   forall se s q, ~ (Smallstep.at_external (L se)) s q. *)
+
+(* Lemma li_null_closed {li} (L: semantics li_null li): lts_closed L. *)
+(* Proof. *)
+(*   unfold lts_closed. *)
+(*   intros. inversion q. *)
+(* Qed. *)
+
+(* Section LTS_CLOSED. *)
+
+(*   Context {liA liB} (L: semantics liA liB). *)
+(*   Context (HL: lts_closed L). *)
+
+(*   Variable liX: language_interface. *)
+(*   Definition lts' se: lts liX liB (state L) := *)
+(*     {| *)
+(*     genvtype := genvtype (L se); *)
+(*     step ge := step (L se) ge; *)
+(*     valid_query := valid_query (L se); *)
+(*     initial_state := initial_state (L se); *)
+(*     at_external := fun s q => False; *)
+(*     after_external := fun q s r => False; *)
+(*     final_state := final_state (L se); *)
+(*     globalenv := globalenv (L se) *)
+(*     |}. *)
+(*   Definition closed_sem_conv := *)
+(*     {| *)
+(*     skel := skel L; *)
+(*     activate se := lts' se; *)
+(*     |}. *)
+
+(*   (* TODO: proved equivalence *) *)
+(* End LTS_CLOSED. *)
+
+
 Require Import CatComp.
 Require Import Linking.
 
-Definition layer_combine {K} (M: Clight.program)
-           (L: Smallstep.semantics li_null (li_c @ K)) sk :=
-  let L' := CatComp.semantics (semantics1 M @ K) (closed_sem_conv L (li_c @ K)) sk
-  in closed_sem_conv L' li_null.
 
-
+Definition layer_combine {K} (M: Clight.program) (L: layer K) sk :=
+  (* let L' := CatComp.semantics (semantics1 M @ K) (closed_sem_conv L (li_c @ K)) sk *)
+  (* in closed_sem_conv L' li_null. *)
+  layer_comp (semantics1 M @ K) L sk.
 Record prog_ksim {K1 K2: Type} :=
   mk_prog_ksim {
-      L1: Smallstep.semantics li_null (li_c @ K1);
-      L2: Smallstep.semantics li_null (li_c @ K2);
+      L1: layer K1;
+      L2: layer K2;
       M: Clight.program;
       R: krel K1 K2;
       sk: AST.program unit unit;
@@ -186,5 +235,22 @@ Section PROG_SIM.
   Qed.
 End PROG_SIM.
 Coercion prog_sim_coercion : prog_ksim >-> Ksim.ksim.
+
+Section VCOMP.
+
+  Context {K1 K2 K3 L1 L2 L3} {M N: Clight.program}
+          {R: krel K1 K2} {S: krel K2 K3} {sk1 sk2}
+          (Hsk1: link (skel L2) (skel (semantics1 M)) = Some sk1)
+          (Hsk2: link (skel L3) (skel (semantics1 N)) = Some sk2)
+          (HL1: forward_simulation 1 (kcc_ext R) L1 (layer_combine M L2 sk1))
+          (HL2: forward_simulation 1 (kcc_ext S) L2 (layer_combine N L3 sk2)).
+  Context (p: Clight.program) (Hlk: link M N = Some p).
+
+  Theorem layer_vcomp:
+    forward_simulation 1 (kcc_ext (krel_comp R S)) L1 (layer_combine p L3 sk2).
+  Proof.
+
+End VCOMP.
+
 
 Require Import FlatComp.
